BinaryHeap/CompleteTree/HeapProofs/HeapUpdateAt.lean
@@ -5,11 +5,12 @@ import BinaryHeap.CompleteTree.HeapProofs.HeapUpdateRoot
 
 namespace BinaryHeap.CompleteTree
 
-private theorem heapUpdateAtIsHeapLeRootAux_RootLeValue {α : Type u} {n : Nat} (le : α → α → Bool) (index : Fin n) (value : α) (heap : CompleteTree α n) (h₁ : HeapPredicate heap le) (h₂ : n > 0) (h₃ : le (root heap h₂) value) (h₄ : total_le le) : HeapPredicate.leOrLeaf le (root heap h₂) (heapUpdateAt le index value heap h₂).fst := by
-  unfold heapUpdateAt
+private theorem heapUpdateAtIsHeapLeRootAux_RootLeValue {α : Type u} {n : Nat} (le : α → α → Bool) (index : Fin n) (value : α) (heap : CompleteTree α n) (h₁ : HeapPredicate heap le) (h₂ : n > 0) (h₃ : le (root heap h₂) value) (h₄ : total_le le) : HeapPredicate.leOrLeaf le (root heap h₂) (heapUpdateAt le index value heap).fst := by
+  unfold heapUpdateAt heapUpdateAtAux
   split
   case isTrue => exact CompleteTree.heapUpdateRootIsHeapLeRootAux le value heap h₁ h₂ h₃
   case isFalse hi =>
+    generalize heapUpdateAt.proof_1 index = h₂
     split
     rename_i o p v l r h₆ h₇ h₈ index h₁ h₅
     cases h₉ : le v value <;> simp (config := { ground := true }) only
@@ -19,8 +20,9 @@ private theorem heapUpdateAtIsHeapLeRootAux_RootLeValue {α : Type u} {n : Nat} 
       split
       <;> simp![reflexive_le, h₄]
 
-private theorem heapUpdateAtIsHeapLeRootAux_ValueLeRoot {α : Type u} {n : Nat} (le : α → α → Bool) (index : Fin n) (value : α) (heap : CompleteTree α n) (h₁ : HeapPredicate heap le) (h₂ : n > 0) (h₃ : le value (root heap h₂)) (h₄ : total_le le) (h₅ : transitive_le le) : HeapPredicate.leOrLeaf le value (heapUpdateAt le index value heap h₂).fst := by
-  unfold heapUpdateAt
+private theorem heapUpdateAtIsHeapLeRootAux_ValueLeRoot {α : Type u} {n : Nat} (le : α → α → Bool) (index : Fin n) (value : α) (heap : CompleteTree α n) (h₁ : HeapPredicate heap le) (h₂ : n > 0) (h₃ : le value (root heap h₂)) (h₄ : total_le le) (h₅ : transitive_le le) : HeapPredicate.leOrLeaf le value (heapUpdateAt le index value heap).fst := by
+  unfold heapUpdateAt heapUpdateAtAux
+  generalize heapUpdateAt.proof_1 index = h₂
   split
   <;> rename_i h₉
   case isTrue =>
@@ -42,11 +44,12 @@ private theorem heapUpdateAtIsHeapLeRootAux_ValueLeRoot {α : Type u} {n : Nat} 
     <;> unfold HeapPredicate.leOrLeaf
     <;> simp only [root_unfold, h₃, h₄, reflexive_le]
 
-theorem heapUpdateAtIsHeap {α : Type u} {n : Nat} (le : α → α → Bool) (index : Fin n) (value : α) (heap : CompleteTree α n) (h₁ : n > 0) (h₂ : HeapPredicate heap le) (h₃ : transitive_le le) (h₄ : total_le le) : HeapPredicate (heap.heapUpdateAt le index value h₁).fst le := by
-  unfold heapUpdateAt
+theorem heapUpdateAtIsHeap {α : Type u} {n : Nat} (le : α → α → Bool) (index : Fin n) (value : α) (heap : CompleteTree α n) (h₂ : HeapPredicate heap le) (h₃ : transitive_le le) (h₄ : total_le le) : HeapPredicate (heap.heapUpdateAt le index value).fst le := by
+  unfold heapUpdateAt heapUpdateAtAux
+  generalize heapUpdateAt.proof_1 index = h₁
   split
   case isTrue h₅ =>
-    exact heapUpdateRootIsHeap le value heap h₁ h₂ h₃ h₄
+    exact heapUpdateRootIsHeap le value heap _ h₂ h₃ h₄
   case isFalse h₅ =>
     split
     rename_i o p v l r h₆ h₇ h₈ index h₁ h₅
@@ -59,11 +62,11 @@ theorem heapUpdateAtIsHeap {α : Type u} {n : Nat} (le : α → α → Bool) (in
       have h₁₀ := not_le_imp_le h₄ v value (Bool.eq_false_iff.mp h₁₀)
       have h₁₄ : p > 0 := by cases p; exact absurd (Nat.lt_succ.mp index.isLt) h; exact Nat.zero_lt_succ _
       apply And.intro <;> try apply And.intro
-      case left => exact heapUpdateAtIsHeap le ⟨index.val - o - 1, _⟩ v r h₁₄ h₂.right.left h₃ h₄
+      case left => exact heapUpdateAtIsHeap le ⟨index.val - o - 1, _⟩ v r h₂.right.left h₃ h₄
       case right.left => exact HeapPredicate.leOrLeaf_transitive h₃ h₁₀ h₂.right.right.left
       case right.right =>
-        have h₁₁: HeapPredicate (heapUpdateAt le ⟨index.val - o - 1, (by omega)⟩ v r h₁₄).fst le :=
-          (heapUpdateAtIsHeap le ⟨index.val - o - 1, (by omega)⟩ v r _ h₂.right.left h₃ h₄)
+        have h₁₁: HeapPredicate (heapUpdateAt le ⟨index.val - o - 1, (by omega)⟩ v r).fst le :=
+          (heapUpdateAtIsHeap le ⟨index.val - o - 1, (by omega)⟩ v r h₂.right.left h₃ h₄)
         cases h₁₂ : le v (r.root h₁₄)
         case false =>
           cases p
@@ -77,11 +80,11 @@ theorem heapUpdateAtIsHeap {α : Type u} {n : Nat} (le : α → α → Bool) (in
       have h₁₀ := not_le_imp_le h₄ v value (Bool.eq_false_iff.mp h₁₀)
       have h₁₄ : o > 0 := by cases o; simp at h₅ h; exact absurd (Fin.val_inj.mp h : index = 0) h₅; exact Nat.zero_lt_succ _
       apply And.intro <;> try apply And.intro
-      case left => exact heapUpdateAtIsHeap le ⟨index.val - 1, _⟩ v l h₁₄ h₂.left h₃ h₄
+      case left => exact heapUpdateAtIsHeap le ⟨index.val - 1, _⟩ v l h₂.left h₃ h₄
       case right.right => exact HeapPredicate.leOrLeaf_transitive h₃ h₁₀ h₂.right.right.right
       case right.left =>
-        have h₁₁: HeapPredicate (heapUpdateAt le ⟨index.val - 1, (_)⟩ v l h₁₄).fst le :=
-          (heapUpdateAtIsHeap le ⟨index.val - 1, (by omega)⟩ v l _ h₂.left h₃ h₄)
+        have h₁₁: HeapPredicate (heapUpdateAt le ⟨index.val - 1, (_)⟩ v l).fst le :=
+          (heapUpdateAtIsHeap le ⟨index.val - 1, (by omega)⟩ v l h₂.left h₃ h₄)
         cases h₁₂ : le v (l.root h₁₄)
         case false =>
           cases o
@@ -94,10 +97,10 @@ theorem heapUpdateAtIsHeap {α : Type u} {n : Nat} (le : α → α → Bool) (in
     case true.isFalse =>
       have h₁₄ : p > 0 := by cases p; exact absurd (Nat.lt_succ.mp index.isLt) h; exact Nat.zero_lt_succ _
       apply And.intro
-      case left => exact heapUpdateAtIsHeap le ⟨index.val - o - 1, _⟩ value r h₁₄ h₂.right.left h₃ h₄
+      case left => exact heapUpdateAtIsHeap le ⟨index.val - o - 1, _⟩ value r h₂.right.left h₃ h₄
       case right =>
-        have h₁₁: HeapPredicate (heapUpdateAt le ⟨index.val - o - 1, (by omega)⟩ v r (h₁₄)).fst le :=
-          (heapUpdateAtIsHeap le ⟨index.val - o - 1, (by omega)⟩ v r _ h₂.right.left h₃ h₄)
+        have h₁₁: HeapPredicate (heapUpdateAt le ⟨index.val - o - 1, (by omega)⟩ v r).fst le :=
+          (heapUpdateAtIsHeap le ⟨index.val - o - 1, (by omega)⟩ v r h₂.right.left h₃ h₄)
         cases h₁₂ : le value (r.root h₁₄)
         case false =>
           have h₁₃ := heapUpdateAtIsHeapLeRootAux_RootLeValue le ⟨index.val - o - 1, (by omega)⟩ value r h₂.right.left (by omega) (not_le_imp_le h₄ value (r.root h₁₄) (Bool.eq_false_iff.mp h₁₂)) h₄
@@ -112,10 +115,10 @@ theorem heapUpdateAtIsHeap {α : Type u} {n : Nat} (le : α → α → Bool) (in
     case true.isTrue =>
       have h₁₄ : o > 0 := by cases o; simp at h₅ h; exact absurd (Fin.val_inj.mp h : index = 0) h₅; exact Nat.zero_lt_succ _
       apply And.intro
-      case left => exact heapUpdateAtIsHeap le ⟨index.val - 1, _⟩ value l h₁₄ h₂.left h₃ h₄
+      case left => exact heapUpdateAtIsHeap le ⟨index.val - 1, _⟩ value l h₂.left h₃ h₄
       case right =>
-        have h₁₁: HeapPredicate (heapUpdateAt le ⟨index.val - 1, (by omega)⟩ v l h₁₄).fst le :=
-          (heapUpdateAtIsHeap le ⟨index.val - 1, (by omega)⟩ v l _ h₂.left h₃ h₄)
+        have h₁₁: HeapPredicate (heapUpdateAt le ⟨index.val - 1, (by omega)⟩ v l).fst le :=
+          (heapUpdateAtIsHeap le ⟨index.val - 1, (by omega)⟩ v l h₂.left h₃ h₄)
         cases h₁₂ : le value (l.root h₁₄)
         case false =>
           have h₁₃ := heapUpdateAtIsHeapLeRootAux_RootLeValue le ⟨index.val - 1, (by omega)⟩ value l h₂.left (by omega) (not_le_imp_le h₄ value (l.root h₁₄) (Bool.eq_false_iff.mp h₁₂)) h₄
